Wavelet/Simulation.lean
@@ -63,37 +63,45 @@ def SimR.varsToChans
       else []
     | _ => []
 
+def SimR.HasMerges
+  (m n : Nat)
+  (atoms : AtomicProcs Op (ChanName χ) V) :
+  List (Bool × ChanName χ) → Prop
+  | [] => True
+  | (_, chan) :: rest =>
+    (compileExpr.brMerge _ _ _ m n chan rest ∈ atoms) ∧
+    SimR.HasMerges m n atoms rest
+
 def SimR
   (hnz : m > 0 ∧ n > 0)
   (ec : Seq.Config Op χ V S m n)
   (pc : Dataflow.Config Op (ChanName χ) V S m n) : Prop :=
   ec.state = pc.state ∧
+  -- Some invariants about the correspondence between variables and channels
+  pc.chans = SimR.varsToChans _ _ _ _ ec ∧
+  ec.definedVars.Nodup ∧
+  (∀ var, var ∈ ec.definedVars ↔ ∃ val, ec.vars.getVar _ _ var = some val) ∧
+  (∀ b var pathConds, (b, .var var pathConds) ∈ ec.pathConds →
+    pathConds.length < ec.pathConds.length) ∧
+  -- Some invariants about the "shape" of the processes
+  SimR.HasMerges _ _ _ m n pc.proc.atoms ec.pathConds ∧
   ∃ (rest : AtomicProcs Op (ChanName χ) V)
     (carryInLoop : Bool)
     (ctxLeft ctxCurrent ctxRight : AtomicProcs Op (ChanName χ) V),
-    -- Some invariants about the "shape" of the processes
     pc.proc.atoms = compileFn.initCarry _ _ _ ec.fn carryInLoop :: rest ∧
     (compileFn Op χ V S hnz ec.fn).atoms = compileFn.initCarry _ _ _ ec.fn false :: rest ∧
     rest = ctxLeft ++ ctxCurrent ++ ctxRight ∧
-    (∀ i, (h : i < ec.pathConds.length) →
-      compileExpr.brMerge _ _ _ m n (ec.pathConds[i]'h).2 (ec.pathConds.drop i) ∈ pc.proc.atoms) ∧
     (∀ vals, ec.expr = .ret vals → ¬ carryInLoop ∧ ctxCurrent = [] ∧ ctxRight = []) ∧
     (∀ expr, ec.expr = .cont expr → carryInLoop ∧
       expr.WellFormed _ _ ec.definedVars ∧
-      compileExpr Op χ V S hnz ec.definedVars ec.pathConds expr = ctxCurrent) ∧
-    -- Some invariants about the correspondence between variables and channels
-    pc.chans = SimR.varsToChans _ _ _ _ ec ∧
-    ec.definedVars.Nodup ∧
-    (∀ var, var ∈ ec.definedVars ↔ ∃ val, ec.vars.getVar _ _ var = some val) ∧
-    (∀ b var pathConds, (b, .var var pathConds) ∈ ec.pathConds →
-      pathConds.length < ec.pathConds.length)
+      compileExpr Op χ V S hnz ec.definedVars ec.pathConds expr = ctxCurrent)
 
-theorem push_vars_lookup_diff
+theorem push_vals_lookup_diff
   {map : ChanMap χ V}
   (hdiff : ∀ v ∈ names, v ≠ name) :
   map.pushVals _ _ names vals name = map name := sorry
 
-theorem push_vars_lookup_singleton
+theorem push_vals_lookup_singleton
   {map : ChanMap χ V}
   {names : Vector χ n}
   (i : Fin n)
@@ -103,47 +111,48 @@ theorem push_vars_lookup_singleton
   (hname : name = names[i]) :
   map.pushVals _ _ names vals name = [val] := sorry
 
-theorem push_var_lookup_diff
+theorem push_val_lookup_diff
   {map : ChanMap χ V}
   (hdiff : name' ≠ name) :
   map.pushVal _ _ name' val name = map name := sorry
 
-theorem push_var_lookup_singleton
+theorem push_val_lookup_singleton
   {map : ChanMap χ V}
   (hempty : map name = []) :
   map.pushVal _ _ name val name = [val] := sorry
 
-theorem pop_vars_lookup_diff
+theorem pop_vals_lookup_diff
   {map : ChanMap χ V}
   (hpop : map.popVals _ _ names = some (vals, map'))
   (hdiff : ∀ v ∈ names, v ≠ name) :
   map' name = map name := sorry
 
-theorem pop_var_lookup_diff
+theorem pop_val_lookup_diff
   {map : ChanMap χ V}
   (hpop : map.popVal _ _ name' = some (val, map'))
   (hdiff : name' ≠ name) :
   map' name = map name := sorry
 
-theorem pop_var_lookup_singleton
+theorem pop_val_lookup_singleton
   {map : ChanMap χ V}
   (hpop : map.popVal _ _ name = some (val, map'))
   (hsingleton : map name = [val]) :
   map' name = [] := sorry
 
-theorem pop_vars_lookup_singleton
+theorem pop_vals_lookup_singleton
   {map : ChanMap χ V}
   (hpop : map.popVals _ _ names = some (val, map'))
   (hmem : name ∈ names)
   (hsingleton : (map name).length = 1) :
   map' name = [] := sorry
 
-theorem pop_singleton
+theorem pop_val_singleton
   {map : ChanMap χ V}
   (hsingleton : map name = [val]) :
-  ∃ map', map.popVal _ _ name = some (val, map') := sorry
+  ∃ map', map.popVal _ _ name = some (val, map') := by
+  simp [ChanMap.popVal, hsingleton]
 
-theorem pops_singleton
+theorem pop_vals_singleton
   {map : ChanMap χ V}
   {names : Vector χ n}
   (prop : χ → V → Prop)
@@ -152,7 +161,46 @@ theorem pops_singleton
     map.popVals _ _ names = some (vals, map') ∧
     List.Forall₂ prop names.toList vals.toList := sorry
 
+theorem pop_val_singleton_rewrite
+  {map : ChanMap χ V}
+  (hsingleton : map name = [val]) :
+  map.popVal _ _ name = some (val, λ n => if n = name then [] else map n) := sorry
+
+theorem pop_vals_singleton_rewrite
+  {map : ChanMap χ V}
+  (prop : χ → V → Prop)
+  (hsingletons : ∀ name ∈ names, ∃ val, map name = [val] ∧ prop name val) :
+  ∃ vals,
+    map.popVals _ _ names = some (vals, λ n => if n ∈ names then [] else map n) ∧
+    List.Forall₂ prop names.toList vals.toList := sorry
+
+theorem sim_step_ret
+  (hnz : m > 0 ∧ n > 0)
+  (ec ec' : Seq.Config Op χ V S m n)
+  (pc : Dataflow.Config Op (ChanName χ) V S m n)
+  (hsim : SimR _ _ _ _ hnz ec pc)
+  (hstep : Config.Step Op χ V S ec ec')
+  (hbr : ec.expr = .cont (.ret vars)) :
+  ∃ pc',
+    Config.StepPlus Op (ChanName χ) V S pc pc' ∧
+    SimR _ _ _ _ hnz ec' pc' := by
+  sorry
+
 set_option maxHeartbeats 300000
+
+-- theorem sim_step_br_chans₃_empty_var
+--   {ec : Seq.Config Op χ V S m n} {cond}
+--   {chans chans₁ chans₂ chans₃ : ChanMap (ChanName χ) V}
+--   {inputVals : Vector V _}
+--   (hchans : chans = SimR.varsToChans _ _ _ _ ec)
+--   (hchans₁ : chans.popVal _ _ condName = some (condVal, chans₁))
+--   (hchans₂ : (chans₁.pushVals _ _
+--     #v[.switch_cond condName, .merge_cond condName]
+--     (Vector.replicate 2 condVal)).popVal _ _ (.switch_cond condName) = some (condVal, chans₂))
+--   (hchans₃ : chans₂.popVals _ _
+--     (compileExpr.allVarsExcept χ ec.definedVars cond ec.pathConds) = some (inputVals, chans₃))
+--   : chans₃ (.var var pathConds) = []
+-- := sorry
 
 theorem sim_step_br
   {cond}
@@ -167,18 +215,18 @@ theorem sim_step_br
     SimR _ _ _ _ hnz ec' pc' := by
   have ⟨
     heq_state,
+    hlive_vars,
+    hdefined_vars_no_dup,
+    hdefined_vars,
+    hpath_conds_order,
+    hmerges,
     ⟨
       rest, carryInLoop, ctxLeft, ctxCurrent, ctxRight,
       hatoms,
       hcomp_fn,
       hrest,
-      hmerges,
       hret,
       hcont,
-      hlive_vars,
-      hdefined_vars_no_dup,
-      hdefined_vars,
-      hpath_conds_order,
     ⟩,
   ⟩ := hsim
   have ⟨hcarryInLoop, hwf_expr, hcurrent⟩ := hcont (.br cond left right) hbr
@@ -194,6 +242,7 @@ theorem sim_step_br
     have heq_cond' := hexpr.1; subst heq_cond'
     have heq_left' := hexpr.2.1; subst heq_left'
     have heq_right' := hexpr.2.2; subst heq_right'
+    clear hexpr
     cases hwf_expr with | wf_br hwf_left hwf_right =>
     -- Some abbreviations
     generalize hcondName :
@@ -210,7 +259,7 @@ theorem sim_step_br
     generalize hrightComp :
       compileExpr Op χ V S hnz (ec.definedVars.erase cond) rightConds right = rightComp
     simp only [hleftComp, hrightComp] at hcurrent
-    -- Step 1: Pop `cond` and run the first `fork`.
+    -- Step 1: Pop `cond` and fire the first `fork`.
     have hcondVal : pc.chans condName = [condVal]
     := by simp [hlive_vars, SimR.varsToChans, hcond, ← hcondName]
     have ⟨chans₁, hchans₁⟩ :
@@ -232,7 +281,7 @@ theorem sim_step_br
       apply step_eq
       apply Dataflow.Config.Step.step_fork hmem_fork hchans₁
       simp [← hpc₁]
-    -- Step 2: Run the switch
+    -- Step 2: Fire the `switch` operator
     have hmem_switch :
       .switch (.switch_cond condName)
         (compileExpr.allVarsExcept χ ec.definedVars cond ec.pathConds)
@@ -244,10 +293,10 @@ theorem sim_step_br
       ∃ chans₂, pc₁.chans.popVal _ _ (.switch_cond condName) = some (condVal, chans₂)
     := by
       simp [← hpc₁]
-      apply pop_singleton
-      rw [push_vars_lookup_singleton _ _ 0]
+      apply pop_val_singleton
+      rw [push_vals_lookup_singleton _ _ 0]
       · simp
-        rw [pop_var_lookup_diff _ _ hchans₁]
+        rw [pop_val_lookup_diff _ _ hchans₁]
         · simp [hlive_vars, SimR.varsToChans]
         · nofun
       · simp
@@ -266,16 +315,16 @@ theorem sim_step_br
           (compileExpr.allVarsExcept χ ec.definedVars cond ec.pathConds).toList
           inputVals.toList
     := by
-      apply pops_singleton
+      apply pop_vals_singleton
       intros name hname
       simp [compileExpr.allVarsExcept] at hname
       replace ⟨var, hvar, hname⟩ := hname
       simp [List.toVector] at hvar
       simp [← hname]
-      rw [pop_var_lookup_diff _ _ hchans₂]
+      rw [pop_val_lookup_diff _ _ hchans₂]
       · simp [← hpc₁]
-        rw [push_vars_lookup_diff]
-        · rw [pop_var_lookup_diff _ _ hchans₁]
+        rw [push_vals_lookup_diff]
+        · rw [pop_val_lookup_diff _ _ hchans₁]
           · simp [hlive_vars, SimR.varsToChans]
             have hmem_var := List.mem_of_mem_erase hvar
             have ⟨_, h⟩ := (hdefined_vars var).mp hmem_var
@@ -293,55 +342,47 @@ theorem sim_step_br
       if heq : ec.pathConds = pathConds then
         if hmem_var : var ∈ ec.definedVars.erase cond then
           -- The popped variable is `cond`
-          rw [pop_vars_lookup_singleton _ _ hchans₃]
-          · simp [← heq, hmem_var, compileExpr.allVarsExcept, List.toVector]
-          · rw [pop_var_lookup_diff _ _ hchans₂]
-            · simp [← hpc₁]
-              rw [push_vars_lookup_diff]
-              · rw [pop_var_lookup_diff _ _ hchans₁]
-                · simp [hlive_vars, SimR.varsToChans, heq]
-                  have ⟨_, h⟩ := (hdefined_vars var).mp (List.mem_of_mem_erase hmem_var)
-                  simp [h]
-                · simp [← hcondName, heq]
-                  have := (List.Nodup.mem_erase_iff hdefined_vars_no_dup).mp hmem_var
-                  intro h
-                  simp [h] at this
-              · simp
-            · simp
+          rw [pop_vals_lookup_singleton _ _ hchans₃
+            (by simp [← heq, hmem_var, compileExpr.allVarsExcept, List.toVector])]
+          rw [pop_val_lookup_diff _ _ hchans₂ (by simp)]
+          simp [← hpc₁]
+          rw [push_vals_lookup_diff _ _ (by simp)]
+          rw [pop_val_lookup_diff _ _ hchans₁]
+          · simp [hlive_vars, SimR.varsToChans, heq]
+            have ⟨_, h⟩ := (hdefined_vars var).mp (List.mem_of_mem_erase hmem_var)
+            simp [h]
+          · simp [← hcondName, heq]
+            have := (List.Nodup.mem_erase_iff hdefined_vars_no_dup).mp hmem_var
+            intro h
+            simp [h] at this
         else
-          rw [pop_vars_lookup_diff _ _ hchans₃]
-          · rw [pop_var_lookup_diff _ _ hchans₂]
-            · simp [← hpc₁]
-              rw [push_vars_lookup_diff]
-              · if heq_cond : cond = var then
-                  simp only [← heq, ← heq_cond, hcondName]
-                  rw [pop_var_lookup_singleton _ _ hchans₁]
-                  simp [hlive_vars, SimR.varsToChans, ← hcondName, hcond]
-                else
-                  rw [pop_var_lookup_diff _ _ hchans₁]
-                  · simp [hlive_vars, SimR.varsToChans, heq]
-                    split
-                    · rename_i h
-                      have := (hdefined_vars var).mpr ⟨_, h⟩
-                      grind only [=_ List.cons_append, = List.append_assoc, = List.nodup_iff_count,
-                        List.mem_erase_of_ne, =_ List.contains_iff_mem, Vector.replicate_succ,
-                        = List.nodup_iff_pairwise_ne, List.mem_cons_of_mem, =_ List.append_assoc,
-                        usr List.length_pos_of_mem, = List.length_erase,
-                        → List.eq_nil_of_append_eq_nil, List.size_toArray, → List.mem_of_mem_erase]
-                    · rfl
-                  · simp [← hcondName, heq_cond]
-              · simp
-            · simp
+          rw [pop_vals_lookup_diff _ _ hchans₃]
+          · rw [pop_val_lookup_diff _ _ hchans₂ (by simp)]
+            simp [← hpc₁]
+            rw [push_vals_lookup_diff _ _ (by simp)]
+            if heq_cond : cond = var then
+              simp only [← heq, ← heq_cond, hcondName]
+              rw [pop_val_lookup_singleton _ _ hchans₁]
+              simp [hlive_vars, SimR.varsToChans, ← hcondName, hcond]
+            else
+              rw [pop_val_lookup_diff _ _ hchans₁ (by simp [← hcondName, heq_cond])]
+              simp [hlive_vars, SimR.varsToChans, heq]
+              split
+              · rename_i h
+                have := (hdefined_vars var).mpr ⟨_, h⟩
+                have := (List.mem_erase_of_ne (Ne.symm heq_cond)).mpr this
+                contradiction
+              · rfl
           · simp [compileExpr.allVarsExcept]
             intros var' hmem_var' h
             simp [h, List.toVector] at hmem_var'
             contradiction
       else
-        rw [pop_vars_lookup_diff _ _ hchans₃]
-        · rw [pop_var_lookup_diff _ _ hchans₂]
+        rw [pop_vals_lookup_diff _ _ hchans₃]
+        · rw [pop_val_lookup_diff _ _ hchans₂]
           · simp [← hpc₁]
-            rw [push_vars_lookup_diff]
-            · rw [pop_var_lookup_diff _ _ hchans₁]
+            rw [push_vals_lookup_diff]
+            · rw [pop_val_lookup_diff _ _ hchans₁]
               · simp only [hlive_vars, SimR.varsToChans]
                 split
                 · rename_i h
@@ -376,6 +417,209 @@ theorem sim_step_br
     simp only [hsteps, true_and]
     and_intros
     · simp [← hpc₂, heq_state]
+    · funext name
+      simp only [← hpc₂, SimR.varsToChans]
+      cases name with
+      | var v pathConds =>
+        simp
+        have :
+          (condValBool, ChanName.var cond ec.pathConds) :: ec.pathConds
+          = if condValBool = true then leftConds else rightConds
+        := by
+          split
+          · simp [← hleftConds, ← hcondName]
+            assumption
+          · simp [← hrightConds, ← hcondName]
+            rename_i h; simp [h]
+        simp only [this.symm]
+        split
+        · rename_i hpath_conds
+          if hmem_v : v ∈ ec.definedVars.erase cond then
+            have ⟨val, hval⟩ := (hdefined_vars v).mp (List.mem_of_mem_erase hmem_v)
+            have ⟨hne_cond, _⟩ := (List.Nodup.mem_erase_iff hdefined_vars_no_dup).mp hmem_v
+            have ⟨i, hi⟩ := List.mem_iff_get.mp hmem_v
+            simp at hi
+            unfold VarMap.removeVar VarMap.getVar
+            simp
+            rw [push_vals_lookup_singleton _ _ i (val := val)]
+            · grind only [VarMap.getVar]
+            · simp only [compileExpr.allVarsExcept]
+              grind
+            · simp [compileExpr.allVarsExcept, Vector.toList, List.toVector]
+              apply (List.nodup_map_iff _).mpr
+              · exact List.Nodup.erase _ hdefined_vars_no_dup
+              · simp [Function.Injective]
+            · simp [compileExpr.allVarsExcept, List.toVector] at hinputVals
+              have ⟨_, h⟩ := (List.forall₂_iff_get).mp hinputVals
+              specialize h i (by simp) (by simp)
+              simp [hi, hval] at h
+              simp [h]
+            · simp [compileExpr.allVarsExcept, List.toVector, hpath_conds]
+              simp [hi]
+          else
+            rw [push_vals_lookup_diff]
+            · simp [hchans₃_no_var]
+              split
+              · rename_i hget_v
+                grind [VarMap.removeVar, VarMap.getVar]
+              · rfl
+            · simp [compileExpr.allVarsExcept]
+              intros v' hmem_v' h
+              simp [h, List.toVector] at hmem_v'
+              contradiction
+        · rename_i hdiff_path_conds
+          rw [push_vals_lookup_diff]
+          · apply hchans₃_no_var
+          · simp [compileExpr.allVarsExcept]
+            grind only
+      | merge_cond name =>
+        cases hname : condName == name
+        simp
+        all_goals
+          simp at hname
+          split -- split on `condValBool`
+          all_goals
+            rename_i hcondValBool
+            simp [hcondValBool]
+        · rw [push_vals_lookup_diff]
+          · rw [pop_vals_lookup_diff _ _ hchans₃]
+            · rw [pop_val_lookup_diff _ _ hchans₂]
+              · simp only [← hpc₁]
+                rw [push_vals_lookup_diff]
+                · rw [pop_val_lookup_diff _ _ hchans₁]
+                  · simp only [← hcondName] at hname
+                    have : name ≠ ChanName.var cond ec.pathConds := by
+                      intros h; exact hname (h.symm)
+                    simp [hlive_vars, SimR.varsToChans, this]
+                  · simp [← hcondName]
+                · simp [hname]
+              · simp
+            · simp [compileExpr.allVarsExcept]
+          · simp [compileExpr.allVarsExcept]
+        -- NOTE: same as above, simplify...
+        · rw [push_vals_lookup_diff]
+          · rw [pop_vals_lookup_diff _ _ hchans₃]
+            · rw [pop_val_lookup_diff _ _ hchans₂]
+              · simp only [← hpc₁]
+                rw [push_vals_lookup_diff]
+                · rw [pop_val_lookup_diff _ _ hchans₁]
+                  · simp only [← hcondName] at hname
+                    have : name ≠ ChanName.var cond ec.pathConds := by
+                      intros h; exact hname (h.symm)
+                    simp [hlive_vars, SimR.varsToChans, this]
+                  · simp [← hcondName]
+                · simp [hname]
+              · simp
+            · simp [compileExpr.allVarsExcept]
+          · simp [compileExpr.allVarsExcept]
+        · simp only [← hcondName] at hname
+          simp [← hname]
+          rw [push_vals_lookup_diff]
+          · rw [pop_vals_lookup_diff _ _ hchans₃]
+            · rw [pop_val_lookup_diff _ _ hchans₂]
+              · simp only [← hpc₁]
+                rw [push_vals_lookup_singleton _ _ 1]
+                · simp
+                  rw [pop_val_lookup_diff _ _ hchans₁]
+                  · simp only [hlive_vars, SimR.varsToChans]
+                    split
+                    · rename_i h
+                      simp only [← hcondName] at h
+                      have := hpath_conds_order true cond ec.pathConds h
+                      simp at this
+                    · split
+                      · rename_i h
+                        simp only [← hcondName] at h
+                        have := hpath_conds_order false cond ec.pathConds h
+                        simp at this
+                      · rfl
+                  · nofun
+                · simp
+                · simp
+                  simp only [← hcondValInterp] at hcondValBool
+                  have := (instInterp.unique_true_val condVal).mp hcondValBool
+                  simp [this]
+                · simp [hname, ← hcondName]
+              · simp
+            · simp [compileExpr.allVarsExcept]
+          · simp [compileExpr.allVarsExcept]
+        -- TODO: mostly the same as above, refactor...
+        · simp only [← hcondName] at hname
+          simp [← hname]
+          rw [push_vals_lookup_diff]
+          · rw [pop_vals_lookup_diff _ _ hchans₃]
+            · split
+              · rename_i h
+                have := hpath_conds_order true cond ec.pathConds h
+                simp at this
+              rw [pop_val_lookup_diff _ _ hchans₂]
+              · simp only [← hpc₁]
+                rw [push_vals_lookup_singleton _ _ 1]
+                · simp
+                  rw [pop_val_lookup_diff _ _ hchans₁]
+                  · simp only [hlive_vars, SimR.varsToChans]
+                    split
+                    · rename_i h
+                      simp only [← hcondName] at h
+                      have := hpath_conds_order true cond ec.pathConds h
+                      simp at this
+                    · split
+                      · rename_i h
+                        simp only [← hcondName] at h
+                        have := hpath_conds_order false cond ec.pathConds h
+                        simp at this
+                      · rfl
+                  · grind only
+                · simp
+                · simp
+                  simp only [← hcondValInterp] at hcondValBool
+                  have := (instInterp.unique_false_val condVal).mp hcondValBool
+                  simp [this]
+                · simp [hname, ← hcondName]
+              · simp
+            · simp [compileExpr.allVarsExcept]
+          · simp [compileExpr.allVarsExcept]
+      | switch_cond v =>
+        simp
+        rw [push_vals_lookup_diff _ _ (by simp [compileExpr.allVarsExcept])]
+        rw [pop_vals_lookup_diff _ _ hchans₃ (by simp [compileExpr.allVarsExcept])]
+        if hv : condName = v then
+          -- rw [pop_val_lookup_singleton _ _ hchans₂]
+          simp only [← hv]
+          rw [pop_val_lookup_singleton _ _ hchans₂]
+          simp only [← hpc₁]
+          rw [push_vals_lookup_singleton _ _ 0]
+          · simp
+            rw [pop_val_lookup_diff _ _ hchans₁]
+            · simp only [hlive_vars, SimR.varsToChans]
+            · simp [← hcondName]
+          · simp
+          · simp
+          · simp
+        else
+          rw [pop_val_lookup_diff _ _ hchans₂]
+          · simp only [← hpc₁]
+            rw [push_vals_lookup_diff]
+            · rw [pop_val_lookup_diff _ _ hchans₁]
+              · simp only [hlive_vars, SimR.varsToChans]
+              · simp [← hcondName]
+            · simp [hv]
+          · simp [hv]
+      | _ =>
+        simp
+        rw [push_vals_lookup_diff _ _ (by simp [compileExpr.allVarsExcept])]
+        rw [pop_vals_lookup_diff _ _ hchans₃ (by simp [compileExpr.allVarsExcept])]
+        rw [pop_val_lookup_diff _ _ hchans₂ (by simp)]
+        simp only [← hpc₁]
+        rw [push_vals_lookup_diff _ _ (by simp)]
+        rw [pop_val_lookup_diff _ _ hchans₁]
+        · simp [hlive_vars, SimR.varsToChans, hbr]
+        · simp [← hcondName]
+    · exact List.Nodup.erase _ hdefined_vars_no_dup
+    · grind [VarMap.getVar, VarMap.removeVar]
+    · grind
+    · grind
+    · simp only [← hpc₂, hmerges]
     · exists rest, carryInLoop
       exists -- ctxLeft
         if condValBool then
@@ -401,243 +645,6 @@ theorem sim_step_br
           rightComp ++ [compileExpr.brMerge Op χ V m n condName ec.pathConds] ++ ctxRight
         else
           [compileExpr.brMerge Op χ V m n condName ec.pathConds] ++ ctxRight
-      and_intros
-      · grind only
-      · grind only
-      · grind only [List.length_cons, =_ List.cons_append, = List.append_assoc, List.length_nil,
-          Array.size_empty, = Vector.toArray_empty, List.nil_append, Vector.replicate_zero,
-          List.append_nil, List.eq_or_mem_of_mem_cons, = List.cons_append, Vector.replicate_succ,
-          List.mem_cons_of_mem, =_ List.append_assoc, List.mem_cons_self,
-          → List.eq_nil_of_append_eq_nil, List.size_toArray, List.mem_append, cases Or]
-      · simp
-        -- TODO: prove after checking that this invariant is enough for .ret
-        sorry
-      · split <;> simp
-      · simp [hcarryInLoop]
-        intros expr hcont'
-        grind only [List.length_cons, =_ List.cons_append, = List.append_assoc, List.length_nil,
-          Array.size_empty, = Vector.toArray_empty, List.nil_append, Vector.replicate_zero,
-          List.eq_or_mem_of_mem_cons, = List.cons_append, Vector.replicate_succ,
-          List.mem_cons_of_mem, =_ List.append_assoc, List.mem_cons_self,
-          → List.eq_nil_of_append_eq_nil, List.size_toArray, List.mem_append, cases Or]
-      · funext name
-        simp only [← hpc₂, SimR.varsToChans]
-        cases name with
-        | var v pathConds =>
-          simp
-          have :
-            (condValBool, ChanName.var cond ec.pathConds) :: ec.pathConds
-            = if condValBool = true then leftConds else rightConds
-          := by
-            split
-            · simp [← hleftConds, ← hcondName]
-              assumption
-            · simp [← hrightConds, ← hcondName]
-              rename_i h; simp [h]
-          simp only [this.symm]
-          split
-          · rename_i hpath_conds
-            if hmem_v : v ∈ ec.definedVars.erase cond then
-              have ⟨val, hval⟩ := (hdefined_vars v).mp (List.mem_of_mem_erase hmem_v)
-              have ⟨hne_cond, _⟩ := (List.Nodup.mem_erase_iff hdefined_vars_no_dup).mp hmem_v
-              have ⟨i, hi⟩ := List.mem_iff_get.mp hmem_v
-              simp at hi
-              unfold VarMap.removeVar VarMap.getVar
-              simp
-              rw [push_vars_lookup_singleton _ _ i (val := val)]
-              · grind only [VarMap.getVar]
-              · simp only [compileExpr.allVarsExcept]
-                grind
-              · simp [compileExpr.allVarsExcept, Vector.toList, List.toVector]
-                apply (List.nodup_map_iff _).mpr
-                · grind only [=_ List.cons_append, = List.append_assoc, = List.nodup_iff_count,
-                  List.mem_erase_of_ne, =_ List.contains_iff_mem, Vector.replicate_succ,
-                  List.Nodup.erase, = List.nodup_iff_pairwise_ne, List.mem_cons_of_mem,
-                  = List.get_eq_getElem, =_ List.append_assoc, usr List.length_pos_of_mem,
-                  = List.length_erase, → List.eq_nil_of_append_eq_nil, List.size_toArray,
-                  → List.mem_of_mem_erase]
-                · simp [Function.Injective]
-              · simp [compileExpr.allVarsExcept, List.toVector] at hinputVals
-                have ⟨_, h⟩ := (List.forall₂_iff_get).mp hinputVals
-                specialize h i (by simp) (by simp)
-                simp [hi, hval] at h
-                simp [h]
-              · simp [compileExpr.allVarsExcept, List.toVector, hpath_conds]
-                simp [hi]
-            else
-              rw [push_vars_lookup_diff]
-              · simp [hchans₃_no_var]
-                split
-                · rename_i hget_v
-                  grind [VarMap.removeVar, VarMap.getVar]
-                · rfl
-              · simp [compileExpr.allVarsExcept]
-                intros v' hmem_v' h
-                simp [h, List.toVector] at hmem_v'
-                contradiction
-          · rename_i hdiff_path_conds
-            rw [push_vars_lookup_diff]
-            · apply hchans₃_no_var
-            · simp [compileExpr.allVarsExcept]
-              grind only
-        | merge_cond name =>
-          cases hname : condName == name
-          simp
-          all_goals
-            simp at hname
-            split -- split on `condValBool`
-            all_goals
-              rename_i hcondValBool
-              simp [hcondValBool]
-          · rw [push_vars_lookup_diff]
-            · rw [pop_vars_lookup_diff _ _ hchans₃]
-              · rw [pop_var_lookup_diff _ _ hchans₂]
-                · simp only [← hpc₁]
-                  rw [push_vars_lookup_diff]
-                  · rw [pop_var_lookup_diff _ _ hchans₁]
-                    · simp only [← hcondName] at hname
-                      have : name ≠ ChanName.var cond ec.pathConds := by
-                        intros h; exact hname (h.symm)
-                      simp [hlive_vars, SimR.varsToChans, this]
-                    · simp [← hcondName]
-                  · simp [hname]
-                · simp
-              · simp [compileExpr.allVarsExcept]
-            · simp [compileExpr.allVarsExcept]
-          -- NOTE: same as above, simplify...
-          · rw [push_vars_lookup_diff]
-            · rw [pop_vars_lookup_diff _ _ hchans₃]
-              · rw [pop_var_lookup_diff _ _ hchans₂]
-                · simp only [← hpc₁]
-                  rw [push_vars_lookup_diff]
-                  · rw [pop_var_lookup_diff _ _ hchans₁]
-                    · simp only [← hcondName] at hname
-                      have : name ≠ ChanName.var cond ec.pathConds := by
-                        intros h; exact hname (h.symm)
-                      simp [hlive_vars, SimR.varsToChans, this]
-                    · simp [← hcondName]
-                  · simp [hname]
-                · simp
-              · simp [compileExpr.allVarsExcept]
-            · simp [compileExpr.allVarsExcept]
-          · simp only [← hcondName] at hname
-            simp [← hname]
-            rw [push_vars_lookup_diff]
-            · rw [pop_vars_lookup_diff _ _ hchans₃]
-              · rw [pop_var_lookup_diff _ _ hchans₂]
-                · simp only [← hpc₁]
-                  rw [push_vars_lookup_singleton _ _ 1]
-                  · simp
-                    rw [pop_var_lookup_diff _ _ hchans₁]
-                    · simp only [hlive_vars, SimR.varsToChans]
-                      split
-                      · rename_i h
-                        simp only [← hcondName] at h
-                        have := hpath_conds_order true cond ec.pathConds h
-                        simp at this
-                      · split
-                        · rename_i h
-                          simp only [← hcondName] at h
-                          have := hpath_conds_order false cond ec.pathConds h
-                          simp at this
-                        · rfl
-                    · nofun
-                  · simp
-                  · simp
-                    simp only [← hcondValInterp] at hcondValBool
-                    have := (instInterp.unique_true_val condVal).mp hcondValBool
-                    simp [this]
-                  · simp [hname, ← hcondName]
-                · simp
-              · simp [compileExpr.allVarsExcept]
-            · simp [compileExpr.allVarsExcept]
-          -- TODO: mostly the same as above, refactor...
-          · simp only [← hcondName] at hname
-            simp [← hname]
-            rw [push_vars_lookup_diff]
-            · rw [pop_vars_lookup_diff _ _ hchans₃]
-              · split
-                · rename_i h
-                  have := hpath_conds_order true cond ec.pathConds h
-                  simp at this
-                rw [pop_var_lookup_diff _ _ hchans₂]
-                · simp only [← hpc₁]
-                  rw [push_vars_lookup_singleton _ _ 1]
-                  · simp
-                    rw [pop_var_lookup_diff _ _ hchans₁]
-                    · simp only [hlive_vars, SimR.varsToChans]
-                      split
-                      · rename_i h
-                        simp only [← hcondName] at h
-                        have := hpath_conds_order true cond ec.pathConds h
-                        simp at this
-                      · split
-                        · rename_i h
-                          simp only [← hcondName] at h
-                          have := hpath_conds_order false cond ec.pathConds h
-                          simp at this
-                        · rfl
-                    · grind only
-                  · simp
-                  · simp
-                    simp only [← hcondValInterp] at hcondValBool
-                    have := (instInterp.unique_false_val condVal).mp hcondValBool
-                    simp [this]
-                  · simp [hname, ← hcondName]
-                · simp
-              · simp [compileExpr.allVarsExcept]
-            · simp [compileExpr.allVarsExcept]
-        | switch_cond v =>
-          simp
-          split
-          all_goals
-            rw [push_vars_lookup_diff]
-            · rw [pop_vars_lookup_diff _ _ hchans₃]
-              · if hv : condName = v then
-                  -- rw [pop_var_lookup_singleton _ _ hchans₂]
-                  simp only [← hv]
-                  rw [pop_var_lookup_singleton _ _ hchans₂]
-                  simp only [← hpc₁]
-                  rw [push_vars_lookup_singleton _ _ 0]
-                  · simp
-                    rw [pop_var_lookup_diff _ _ hchans₁]
-                    · simp only [hlive_vars, SimR.varsToChans]
-                    · simp [← hcondName]
-                  · simp
-                  · simp
-                  · simp
-                else
-                  rw [pop_var_lookup_diff _ _ hchans₂]
-                  · simp only [← hpc₁]
-                    rw [push_vars_lookup_diff]
-                    · rw [pop_var_lookup_diff _ _ hchans₁]
-                      · simp only [hlive_vars, SimR.varsToChans]
-                      · simp [← hcondName]
-                    · simp [hv]
-                  · simp [hv]
-              · simp [compileExpr.allVarsExcept]
-            · simp [compileExpr.allVarsExcept]
-        | _ =>
-          simp
-          split
-          all_goals
-            rw [push_vars_lookup_diff]
-            · rw [pop_vars_lookup_diff _ _ hchans₃]
-              · rw [pop_var_lookup_diff _ _ hchans₂]
-                · simp only [← hpc₁]
-                  rw [push_vars_lookup_diff]
-                  · rw [pop_var_lookup_diff _ _ hchans₁]
-                    · simp only [hlive_vars, SimR.varsToChans, hbr]
-                    · simp [← hcondName]
-                  · simp
-                · simp
-              · simp [compileExpr.allVarsExcept]
-            · simp [compileExpr.allVarsExcept]
-      · grind only [=_ List.cons_append, = List.append_assoc, = List.nodup_iff_count,
-          Vector.replicate_succ, List.Nodup.erase, = List.nodup_iff_pairwise_ne,
-          List.mem_cons_of_mem, =_ List.append_assoc, = List.length_erase,
-          → List.eq_nil_of_append_eq_nil, List.size_toArray]
-      · grind [VarMap.getVar, VarMap.removeVar]
-      · grind
+      grind
 
 end Wavelet.Simulation
